src/tactic/fol/pull.lean
@@ -57,23 +57,53 @@ by { rw ← neg_eqv_neg,
      simp only [form₂.neg, neg_incr,
      bnot, pull_fa_left_eqv] }
 
-
 def pull_left_eqv [inhabited α] (ae ao : bool) (p q : form₂) :
   form₂.qua ae (form₂.bin ao p q.incr) <==α==>
   form₂.bin ao (form₂.qua ae p) q :=
 by {cases ae, apply pull_fa_left_eqv, apply pull_ex_left_eqv }
 
--- def pull_right_eqv [inhabited α] (ae ao : bool) (p q : form₂) :
---   form₂.qua ae (form₂.bin ao p.incr q) <==α==>
---   form₂.bin ao p (form₂.qua ae q) :=
--- begin
---   have h0 : ( form₂.qua ae (form₂.bin ao (form₂.incr p) q) <==α==>
---               form₂.qua ae (form₂.bin ao q (form₂.incr p)) ) :=
---   qua_eqv_qua (bin_comm _ _ _),
---   intro M,
---   simp only [ h0 M, pull_left_eqv ae ao q p M,
---     bin_comm ao p (form₂.qua ae q) M ]
--- end
+def pull_right_eqv [inhabited α] (ae ao : bool) (p q : form₂) :
+  form₂.qua ae (form₂.bin ao p.incr q) <==α==>
+  form₂.bin ao p (form₂.qua ae q) :=
+begin
+  have h0 : ( form₂.qua ae (form₂.bin ao (form₂.incr p) q) <==α==>
+              form₂.qua ae (form₂.bin ao q (form₂.incr p)) ) :=
+  qua_eqv_qua (bin_comm _ _ _),
+  intro M,
+  simp only [ h0 M, pull_left_eqv ae ao q p M,
+    bin_comm ao p (form₂.qua ae q) M ]
+end
+
+--def pull' (b : bool) : form₂ → form₂ → form₂
+--| p ⟪b, t⟫            := form₂.bin b p ⟪b, t⟫
+--| p (form₂.bin c q r) := form₂.bin b p (form₂.bin c q r)
+--| p (form₂.qua c q)   := form₂.qua c (pull' p.incr q)
+--
+--/- Pull all quantifiers over a binary connective.
+--   `b` specifies the binary connective. -/
+--def pull (b : bool) : form₂ → form₂ → form₂
+--| ⟪c, t⟫            q := pull' b ⟪c, t⟫ q
+--| (form₂.bin c p q) r := pull' b (form₂.bin c p q) r
+--| (form₂.qua c p)   q := form₂.qua c (pull p q.incr)
+
+def pull' (o : option bool) (a : bool) : form₂ → form₂ → form₂
+| p ⟪b, t⟫            := form₂.bin a p ⟪b, t⟫
+| p (form₂.bin c q r) := form₂.bin a p (form₂.bin c q r)
+| p (form₂.qua c q)   :=
+  if (some $ bnot c) = o
+  then form₂.bin a p (form₂.qua c q)
+  else form₂.qua c (pull' p.incr q)
+
+/- Pull quantifiers over a binary connective.
+   'o' specifies the polairy of quantifiers being
+   pulled, `b` specifies the binary connective. -/
+def pull (o : option bool) (b : bool) : form₂ → form₂ → form₂
+| ⟪c, t⟫            q := pull' o b ⟪c, t⟫ q
+| (form₂.bin c p q) r := pull' o b (form₂.bin c p q) r
+| (form₂.qua c p)   q :=
+  if (some $ bnot c) = o
+  then pull' o b (form₂.qua c p) q
+  else form₂.qua c (pull p q.incr)
 
 @[reducible] def form₂.size_of_ordered :
   (Σ' (b : bool), (Σ' (a : form₂), form₂)) → nat
@@ -85,263 +115,186 @@ meta def form₂.show_size_lt : tactic unit :=
    nat.lt_succ_self, add_comm, add_lt_add_iff_left,
    add_left_comm, form₂.size_of_incr ] ]
 
-/- Pull quantifiers over a binary connective. `ae` specifies
-   the type of quantifier to be pulled, and `ao` specifies
-   the binary connective. -/
-def pull (ae : option bool) (ao : bool) : bool → form₂ → form₂ → form₂
-| tt (form₂.qua b p) q :=
-  have form₂.size_of_ordered ⟨ff, ⟨q, form₂.qua b p⟩⟩ <
-       form₂.size_of_ordered ⟨tt, ⟨form₂.qua b p, q⟩⟩,
-  by form₂.show_size_lt,
-  if ae = some (bnot b)
-  then pull ff q (form₂.qua b p)
-  else form₂.qua b (pull tt p q.incr)
-| ff (form₂.qua b p) q :=
-  have form₂.size_of_ordered ⟨ff, ⟨p, form₂.incr q⟩⟩ <
-       form₂.size_of_ordered ⟨ff, ⟨form₂.qua b p, q⟩⟩,
-  by form₂.show_size_lt,
-  if ae = some (bnot b)
-  then form₂.bin ao (form₂.qua b p) q
-  else form₂.qua b (pull ff p q.incr)
-| tt p q :=
-  have form₂.size_of_ordered ⟨ff, ⟨q, p⟩⟩ <
-       form₂.size_of_ordered ⟨tt, ⟨p, q⟩⟩,
-  by form₂.show_size_lt,
-  pull ff q p
-| ff p q := form₂.bin ao p q
-using_well_founded
-  {rel_tac := λ _ _, `[exact ⟨_, measure_wf form₂.size_of_ordered⟩]}
+lemma fov_pull' (o : option bool) (b : bool) :
+  ∀ {p q : form₂} {k : nat},
+  p.fov k → q.fov k → (pull' o b p q).fov k
+| p ⟪b, t⟫            k h0 h1 := ⟨h0, h1⟩
+| p (form₂.bin c q r) k h0 h1 := ⟨h0, h1⟩
+| p (form₂.qua c q)   k h0 h1 :=
+  by { apply ite_cases,
+       refine ⟨h0, h1⟩,
+       apply fov_pull' (fov_incr h0) h1 }
 
-lemma fov_pull (ae : option bool) (ao : bool) :
-  ∀ (ls : bool) {p q : form₂} {k : nat},
-  p.fov k → q.fov k → (pull ae ao ls p q).fov k
-| tt ⟪m, a⟫           q :=
-  have 0 < form₂.size_of ⟪m,a⟫ := zero_lt_one,
-  by { intros k h0 h1,
-       unfold pull,
-       apply fov_pull ff h1 h0 }
-| ff ⟪m, a⟫           q :=
-  by { intros k h0 h1,
-       unfold pull,
-       refine ⟨h0, h1⟩ }
-| tt (form₂.bin b p q) r :=
-  have form₂.size_of_ordered ⟨ff, ⟨r, form₂.bin b p q⟩⟩ <
-       form₂.size_of_ordered ⟨tt, ⟨form₂.bin b p q, r⟩⟩,
-  by form₂.show_size_lt,
-  by { intros k h0 h1,
-       unfold pull,
-       apply fov_pull ff h1 h0 }
-| ff (form₂.bin b p q) r :=
-  by { intros k h0 h1,
-       unfold pull,
-       refine ⟨h0, h1⟩ }
-| tt (form₂.qua b p)   q :=
-  have form₂.size_of_ordered ⟨ff, ⟨q, form₂.qua b p⟩⟩ <
-       form₂.size_of_ordered ⟨tt, ⟨form₂.qua b p, q⟩⟩,
-  by form₂.show_size_lt,
+lemma fov_pull (o : option bool) (b : bool) :
+  ∀ {p q : form₂} {k : nat},
+  p.fov k → q.fov k → (pull o b p q).fov k
+| ⟪c, t⟫            q k h0 h1 := fov_pull' _ _ h0 h1
+| (form₂.bin c p q) r k h0 h1 := fov_pull' _ _ h0 h1
+| (form₂.qua c p)   q k h0 h1 :=
+  by { apply ite_cases,
+       { apply fov_pull' _ _ h0 h1 },
+       apply fov_pull _ (fov_incr h1),
+       exact h0 }
+
+-- lemma fov_pull' (a : bool) :
+--   ∀ {p q : form₂} {k : nat},
+--   p.fov k → q.fov k → (pull' a p q).fov k
+-- | p ⟪b, t⟫            k h0 h1 := ⟨h0, h1⟩
+-- | p (form₂.bin b q r) k h0 h1 := ⟨h0, h1⟩
+-- | p (form₂.qua b q)   k h0 h1 :=
+--   @fov_pull' p.incr q (k + 1) (fov_incr h0) h1
+--
+-- lemma fov_pull (b : bool) :
+--   ∀ {p q : form₂} {k : nat},
+--   p.fov k → q.fov k → (pull b p q).fov k
+-- | ⟪c, t⟫            q k h0 h1 := fov_pull' _ h0 h1
+-- | (form₂.bin c p q) r k h0 h1 := fov_pull' _ h0 h1
+-- | (form₂.qua c p)   q k h0 h1 :=
+--   @fov_pull p q.incr (k + 1) h0 (fov_incr h1)
+
+lemma foq_pull' (o : option bool) (a b : bool) :
+  ∀ {p q : form₂}, foq a p → foq a q → foq a (pull' o b p q)
+| p ⟪b, t⟫            h0 h1 := ⟨h0, h1⟩
+| p (form₂.bin b q r) h0 h1 := ⟨h0, h1⟩
+| p (form₂.qua b q)   h0 h1 :=
   begin
-    intros k h0 h1,
-    unfold pull,
-    apply ite_cases,
-    { apply fov_pull ff h1 h0 },
-    apply fov_pull,
-    { apply h0 },
-    apply fov_incr h1
-  end
-| ff (form₂.qua b p)   q :=
-  have form₂.size_of_ordered ⟨ff, ⟨p, form₂.incr q⟩⟩ <
-       form₂.size_of_ordered ⟨ff, ⟨form₂.qua b p, q⟩⟩,
-  by form₂.show_size_lt,
-  begin
-    intros k h0 h1,
-    unfold pull,
     apply ite_cases,
     { refine ⟨h0, h1⟩ },
-    apply fov_pull,
-    { apply h0 },
-    apply fov_incr h1
-  end
-using_well_founded
-  { rel_tac := λ _ _, `[exact ⟨_, measure_wf form₂.size_of_ordered⟩] }
-
-lemma foq_pull (ae : option bool) (ao b : bool) :
-  ∀ ls : bool, ∀ {p q : form₂},
-  foq b p → foq b q → foq b (pull ae ao ls p q)
-| tt ⟪m, a⟫           q :=
-  have 0 < form₂.size_of ⟪m,a⟫ := zero_lt_one,
-  by { intros h0 h1,
-       unfold pull,
-       apply foq_pull _ h1 h0 }
-| ff ⟪m, a⟫           q :=
-  by { intros h0 h1,
-       unfold pull,
-       refine ⟨h0, h1⟩ }
-| tt (form₂.bin b p q) r :=
-  have form₂.size_of_ordered ⟨ff, ⟨r, form₂.bin b p q⟩⟩ <
-       form₂.size_of_ordered ⟨tt, ⟨form₂.bin b p q, r⟩⟩,
-  by form₂.show_size_lt,
-  by { intros h0 h1,
-       unfold pull,
-       apply foq_pull _ h1 h0 }
-| ff (form₂.bin b p q) r :=
-  by { intros h0 h1,
-       unfold pull,
-       refine ⟨h0, h1⟩ }
-| tt (form₂.qua b p)   q :=
-  have form₂.size_of_ordered ⟨ff, ⟨q, form₂.qua b p⟩⟩ <
-       form₂.size_of_ordered ⟨tt, ⟨form₂.qua b p, q⟩⟩,
-  by form₂.show_size_lt,
-  begin
-    intros h0 h1,
-    unfold pull,
-    apply ite_cases,
-    { apply foq_pull _ h1 h0 },
-    refine ⟨λ h2, _, _⟩,
-    { subst h2,
-      apply fov_pull _ _ _ (h0.left rfl),
+    constructor,
+    { intro h2,
+      apply fov_pull' _ _ _ (h1.left h2),
       apply form₂.fov_of_not_occ,
       apply form₂.not_occ_incr_ge },
-    apply foq_pull _ h0.right,
-    apply foq_incr_ge h1
+    apply foq_pull' _ h1.right,
+    apply foq_incr_ge h0,
   end
-| ff (form₂.qua c p)   q :=
-  have form₂.size_of_ordered ⟨ff, ⟨p, form₂.incr q⟩⟩ <
-       form₂.size_of_ordered ⟨ff, ⟨form₂.qua b p, q⟩⟩,
-  by form₂.show_size_lt,
+
+-- lemma foq_pull' (a b : bool) :
+--   ∀ {p q : form₂}, foq a p → foq a q → foq a (pull' b p q)
+-- | p ⟪b, t⟫            h0 h1 := ⟨h0, h1⟩
+-- | p (form₂.bin b q r) h0 h1 := ⟨h0, h1⟩
+-- | p (form₂.qua b q)   h0 h1 :=
+--   begin
+--     constructor,
+--     { intro h2,
+--       apply fov_pull' _ _ (h1.left h2),
+--       apply form₂.fov_of_not_occ,
+--       apply form₂.not_occ_incr_ge },
+--     apply foq_pull' _ h1.right,
+--     apply foq_incr_ge h0
+--   end
+
+lemma foq_pull (o : option bool) (a b : bool) :
+  ∀ {p q : form₂}, foq a p → foq a q → foq a (pull o b p q)
+| ⟪c, t⟫            q h0 h1 := foq_pull' _ _ _ h0 h1
+| (form₂.bin c p q) r h0 h1 := foq_pull' _ _ _ h0 h1
+| (form₂.qua c p)   q h0 h1 :=
   begin
-    intros h0 h1,
-    unfold pull,
     apply ite_cases,
-    { refine ⟨h0, h1⟩ },
-    refine ⟨λ h2, _, _⟩,
-    { subst h2,
-      apply fov_pull _ _ _ (h0.left rfl),
+    { apply foq_pull' _ _ _ h0 h1 },
+    constructor,
+    { intro h2,
+      apply fov_pull _ _  (h0.left h2),
       apply form₂.fov_of_not_occ,
       apply form₂.not_occ_incr_ge },
-    apply foq_pull _ h0.right,
-    apply foq_incr_ge h1
+    apply foq_pull h0.right (foq_incr_ge h1),
   end
-using_well_founded
-  { rel_tac := λ _ _, `[exact ⟨_, measure_wf form₂.size_of_ordered⟩] }
 
-def pull_eqv [inhabited α] (ae : option bool) (ao : bool) :
-  ∀ ls : bool, ∀ p q : form₂,
-  pull ae ao ls p q <==α==> form₂.bin ao p q
-| tt ⟪k, a⟫           q :=
-  have 0 < form₂.size_of ⟪k,a⟫ := zero_lt_succ _,
-  by { apply eqv_trans _ (bin_comm _ _ _),
-       unfold pull,
-       apply pull_eqv }
-| ff ⟪k, a⟫           q := by {unfold pull, apply eqv_refl}
-| tt (form₂.bin b p q) r :=
-  have form₂.size_of_ordered ⟨ff, ⟨r, form₂.bin b p q⟩⟩ <
-       form₂.size_of_ordered ⟨tt, ⟨form₂.bin b p q, r⟩⟩,
-  by form₂.show_size_lt,
-  by { apply eqv_trans _ (bin_comm _ _ _),
-       unfold pull,
-       apply pull_eqv }
-| ff (form₂.bin b p q) r := by {unfold pull, apply eqv_refl}
-| tt (form₂.qua b p) q :=
-  have  form₂.size_of_ordered ⟨ff, ⟨q, form₂.qua b p⟩⟩ <
-        form₂.size_of_ordered ⟨tt, ⟨form₂.qua b p, q⟩⟩,
-  by form₂.show_size_lt,
+def pull'_eqv [inhabited α] (o : option bool) (a : bool) :
+  ∀ p q : form₂, pull' o a p q <==α==> form₂.bin a p q
+| p ⟪c, t⟫            := eqv_refl α _
+| p (form₂.bin b q r) := eqv_refl α _
+| p (form₂.qua b q)   :=
   begin
-    unfold pull,
-    apply @ite_cases _ (λ x, x <==α==>form₂.bin ao (form₂.qua b p) q),
-    { apply eqv_trans _ (bin_comm _ _ _),
-      apply pull_eqv },
-    apply eqv_trans
-      (qua_eqv_qua $ pull_eqv _ p _)
-      (pull_left_eqv _ _ _ _)
-  end
-| ff (form₂.qua b p) q :=
-  have  form₂.size_of_ordered ⟨ff, ⟨p, form₂.incr q⟩⟩ <
-        form₂.size_of_ordered ⟨ff, ⟨form₂.qua b p, q⟩⟩,
-  by form₂.show_size_lt,
-  begin
-    unfold pull,
-    apply @ite_cases _ (λ x, x <==α==>form₂.bin ao (form₂.qua b p) q),
+    unfold pull',
+    apply @ite_cases _ (λ x, x <==α==> form₂.bin a p (form₂.qua b q)),
     { apply eqv_refl },
     apply eqv_trans
-      (qua_eqv_qua $ pull_eqv _ p _)
-      (pull_left_eqv _ _ _ _),
+      (qua_eqv_qua $ pull'_eqv p.incr q)
+      (pull_right_eqv _ _ _ _)
   end
-using_well_founded
-  {rel_tac := λ _ _, `[exact ⟨_, measure_wf form₂.size_of_ordered⟩]}
 
-lemma QN_pull_aux {b : bool} (ao : bool) :
-  ∀ {p q : form₂}, p.QN b → q.N b →
-  (pull (some b) ao ff p q).QN b
-| (form₂.lit c a) q h0 h1 :=
-  by {unfold pull, refine ⟨h0, h1⟩}
-| (form₂.bin c p q) r h0 h1 :=
-  by {unfold pull, refine ⟨h0, h1⟩}
-| (form₂.qua c p) q h0 h1 :=
+def pull_eqv [inhabited α] (o : option bool) (a : bool) :
+  ∀ p q : form₂, pull o a p q <==α==> form₂.bin a p q
+| ⟪b, t⟫            q := pull'_eqv o a _ _
+| (form₂.bin b p q) r := pull'_eqv o a _ _
+| (form₂.qua b p)   q :=
   begin
     unfold pull,
-    by_cases h2 : b = bnot c,
+    apply @ite_cases _ (λ x, x <==α==> form₂.bin a (form₂.qua b p) q),
+    { apply pull'_eqv },
+    apply eqv_trans
+      (qua_eqv_qua $ pull_eqv p q.incr)
+      (pull_left_eqv _ _ _ _)
+  end
+
+open form₂
+
+lemma QN_pull' (a b : bool) :
+  ∀ {p q : form₂}, p.N a → q.QN a →
+  (pull' (some a) b p q).QN a
+| p ⟪c, t⟫ h0 h1      := ⟨h0, h1⟩
+| p (bin c q r) h0 h1 := ⟨h0, h1⟩
+| p (qua c q)  h0 h1 :=
+  begin
+    unfold pull',
+    by_cases h2 : a = bnot c,
     { rw [← h2, if_pos rfl],
       rw eq_bnot_iff_ne at h2,
-      refine ⟨⟨h2, h0.right h2⟩, h1⟩ },
+      refine ⟨h0, ⟨h2, h1.right h2⟩⟩ },
     rw if_neg,
-    { have h3 : b = c,
+    { have h3 : a = c,
       { rw eq_bnot_iff_ne at h2,
         apply not_not.elim_left h2 },
       refine ⟨λ _, _, λ h4, absurd h3 h4⟩,
-      apply QN_pull_aux (h0.left h3),
-      apply form₂.N_incr_ge _ h1 },
-    rw option.some_inj, exact h2
+      apply QN_pull' _ (h1.left h3),
+      apply N_incr_ge _ h0 },
+    rw option.some_inj,
+    intro h3, cases (h2 h3.symm)
   end
 
-lemma QN_pull {b : bool} (ao : bool) :
-  ∀ {p q : form₂}, p.QN b → q.QN b →
-  (pull (some b) ao tt p q).QN b
-| (form₂.lit c a) q h0 h1 :=
-  by {unfold pull, apply QN_pull_aux _ h1 h0}
-| (form₂.bin _ p q) r h0 h1 :=
-  by {unfold pull, apply QN_pull_aux _ h1 h0}
-| (form₂.qua c p) q h0 h1 :=
+lemma QN_pull (a b : bool) :
+  ∀ {p q : form₂}, p.QN a → q.QN a →
+  (pull (some a) b p q).QN a
+| ⟪c, t⟫ q h0 h1      := QN_pull' _ _ h0 h1
+| (bin _ p q) r h0 h1 := QN_pull' _ _ h0 h1
+| (qua c p) q h0 h1 :=
   begin
     unfold pull,
-    by_cases h2 : b = bnot c,
+    by_cases h2 : a = bnot c,
     { rw [← h2, if_pos rfl],
       rw eq_bnot_iff_ne at h2,
-      apply QN_pull_aux _ h1,
+      apply QN_pull' _ _ _ h1,
       refine ⟨h2, h0.right h2⟩ },
     rw if_neg,
     { rw [eq_bnot_iff_ne, not_not] at h2,
       refine ⟨λ _, _, λ h3, absurd h2 h3⟩,
       apply QN_pull (h0.left h2),
       apply form₂.QN_incr_ge _ h1 },
-    rw option.some_inj, exact h2
+    rw option.some_inj,
+    intro h3, cases h2 h3.symm
   end
 
-lemma QF_pull_aux {b : bool} (ao : bool) :
-  ∀ {p q : form₂}, p.QF b → q.F →
-  (pull none ao ff p q).QF b
-| (form₂.lit c a)   q h0 h1 :=
-  by {unfold pull, refine ⟨h0, h1⟩}
-| (form₂.bin c p q) r h0 h1 :=
-  by {unfold pull, refine ⟨h0, h1⟩}
-| (form₂.qua c p) q h0 h1 :=
+lemma QF_pull' (a b : bool) :
+  ∀ {p q : form₂}, p.F → q.QF a →
+  (pull' none b p q).QF a
+| p ⟪c, t⟫      h0 h1 := ⟨h0, h1⟩
+| p (bin c q r) h0 h1 := ⟨h0, h1⟩
+| p (qua c q)   h0 h1 :=
   begin
-    unfold pull, rw if_neg,
-    { refine ⟨h0.left,
-        QF_pull_aux h0.right (form₂.F_incr_ge _ h1)⟩ },
-    rintro ⟨_⟩,
+    unfold pull', rw if_neg,
+    { refine ⟨h1.left, QF_pull' (F_incr_ge _ h0) h1.right⟩ },
+    rintro ⟨_⟩
   end
 
 lemma QF_pull {b : bool} (ao : bool) :
   ∀ {p q : form₂}, p.QF b → q.QF b →
-  (pull none ao tt p q).QF b
-| (form₂.lit c a) q h0 h1 :=
-  by {unfold pull, apply QF_pull_aux _ h1 h0 }
-| (form₂.bin _ p q) r h0 h1 :=
-  by {unfold pull, apply QF_pull_aux _ h1 h0 }
-| (form₂.qua c p) q h0 h1 :=
+  (pull none ao  p q).QF b
+| ⟪_, _⟫      q h0 h1 := QF_pull' _ _ h0 h1
+| (bin _ _ _) q h0 h1 := QF_pull' _ _ h0 h1
+| (qua c p) q h0 h1 :=
   begin
     unfold pull, rw if_neg,
-    { refine ⟨h0.left,
-        QF_pull h0.right (form₂.QF_incr_ge _ h1)⟩ },
+    { refine ⟨h0.left, QF_pull h0.right (form₂.QF_incr_ge _ h1)⟩ },
     intro h2, cases h2
   end
