src/tactic/fol/attempt.lean
@@ -1,0 +1,19 @@
+universe u
+
+class inductive attempt (p : Prop)
+| shown (h : p) : attempt
+| unknown       : attempt
+
+def is_shown (c : Prop) [h : attempt c] : Prop :=
+attempt.rec_on h (λ _, true) false --true false
+
+def of_is_shown {c : Prop} [h₁ : attempt c] (h₂ : is_shown c) : c :=
+begin
+  unfold is_shown at h₂,
+  tactic.unfreeze_local_instances,
+  cases h₁, apply h₁, cases h₂
+end
+
+@[reducible]
+def attempt_pred {α : Sort u} (r : α → Prop) :=
+Π (a : α), attempt (r a)
