src/tactic/fol/tests2.lean
@@ -1,0 +1,109 @@
+
+import .main tactic.finish
+
+meta def x01 : expr := `(forall A B C D : Prop, ¬ A → A → C)
+meta def x02 : expr := `(forall A B C D : Prop, (A ∧ A ∧ B) → (A ∧ C ∧ B) → A)
+meta def x03 : expr := `(forall A B C D : Prop, A → ¬ B → ¬ (A → B))
+meta def x04 : expr := `(forall A B C D : Prop, A ∨ B → B ∨ A)
+meta def x05 : expr := `(forall A B C D : Prop, A ∧ B → B ∧ A)
+meta def x06 : expr := `(forall A B C D : Prop, A → (A → B) → (B → C) → C)
+meta def x07 : expr := `(forall A B C D : Prop, (A ∧ B) → (C ∧ B) → C)
+meta def x08 : expr := `(forall A B C D : Prop, A → B → C → D → (A ∧ B) ∧ (C ∧ D))
+meta def x09 : expr := `(forall A B C D : Prop, (A ∧ B) → (B ∧ ¬ C) → A ∨ C)
+meta def x10 : expr := `(forall A B C D : Prop, (A → B) ∧ (B → C) → A → C)
+meta def x11 : expr := `(forall A B C D : Prop, (A → B) ∨ (B → A))
+meta def x12 : expr := `(forall A B C D : Prop, ((A → B) → A) → A)
+meta def x13 : expr := `(forall A B C D : Prop, A → ¬ B → ¬ (A → B))
+meta def x14 : expr := `(forall A B C D : Prop, ¬ (A ↔ ¬ A))
+meta def x15 : expr := `(forall A B C D : Prop, (A ↔ B) -> (A ∧ B → C) → (¬ A ∧ ¬ B → C) → C)
+meta def x16 : expr := `(forall A B C D : Prop, (A ↔ B) -> ((A ∧ ¬ B) ∨ (¬ A ∧ B)) → C)
+meta def x17 : expr := `(forall A B C D : Prop, (A → B) → A → B)
+meta def x18 : expr := `(forall A B C D : Prop, (A → B) → (B → C) → A → C)
+meta def x19 : expr := `(forall A B C D : Prop, (A → B ∨ C) → (B → D) → (C → D) → A → D)
+meta def x20 : expr := `(forall A B C D : Prop, A ∨ B → B ∨ A)
+
+meta def x21 : expr := `(forall (X : Type) (P Q R : X → Prop) (T : X → X → Prop) (a b : X) (h : inhabited X), (∀ x, P x → Q x) → (∀ x, P x) → Q a)
+meta def x22 : expr := `(forall (X : Type) (P Q R : X → Prop) (T : X → X → Prop) (a b : X) (h : inhabited X), (∀ x, P x → Q x) → P a → Q a)
+meta def x23 : expr := `(forall (X : Type) (P Q R : X → Prop) (T : X → X → Prop) (a b : X) (h : inhabited X), ∀ a b, P a → P b → ∃ x, P x)
+meta def x24 : expr := `(forall (X : Type) (P Q R : X → Prop) (T : X → X → Prop) (a b : X) (h : inhabited X), P a → P b → Q b → ∃ x, P x ∧ Q x)
+meta def x25 : expr := `(forall (X : Type) (P Q R : X → Prop) (T : X → X → Prop) (a b : X) (h : inhabited X), P b → Q b → P a → ∃ x, P x ∧ Q x)
+meta def x26 : expr := `(forall (X : Type) (P Q R : X → Prop) (T : X → X → Prop) (a b : X) (h : inhabited X), (∀ x, P x → Q x ∧ R x) → (∀ x, P x → R x ∧ Q x))
+meta def x27 : expr := `(forall (X : Type) (P Q R : X → Prop) (T : X → X → Prop) (a b : X) (h : inhabited X), (∃ x, P x ∧ Q x) → ∃ x, Q x ∧ P x)
+meta def x28 : expr := `(forall (X : Type) (P Q R : X → Prop) (T : X → X → Prop) (a b : X) (h : inhabited X), ∃ x : X, (P x → (∀ y : X, P y)))
+meta def x29 : expr := `(forall (X : Type) (P Q R : X → Prop) (T : X → X → Prop) (a b : X) (h : inhabited X), (∃ x : X, x = x) → ∃ x, ((∃ y, P y) → P x))
+meta def x30 : expr := `(forall (X : Type) (P Q R : X → Prop) (T : X → X → Prop) (a b : X) (h : inhabited X), (∃ x, ∀ y, T x y) → ∀ y, ∃ x, T x y)
+
+meta def x31 : expr := `(forall (a b c d : Prop), a ∧ b → a)
+meta def x32 : expr := `(forall (a b c d : Prop), a → (a → b) → (b → c) ∧ (d → ¬ c) → ¬ d)
+meta def x33 : expr := `(forall (a b c d : Prop), a ∨ b → b ∨ a)
+meta def x34 : expr := `(forall (a b c d : Prop), ¬ (a ↔ ¬ a))
+
+meta def x35 : expr := `(forall (a b c : ℕ) (p q : ℕ → Prop) (r : ℕ → ℕ → Prop) (P Q R : Prop) (g : bool → nat), (∀ x, p x → q x) → (∀ x, p x) → q a)
+meta def x36 : expr := `(forall (a b c : ℕ) (p q : ℕ → Prop) (r : ℕ → ℕ → Prop) (P Q R : Prop) (g : bool → nat), (p a) → ∃ x, p x)
+meta def x37 : expr := `(forall (a b c : ℕ) (p q : ℕ → Prop) (r : ℕ → ℕ → Prop) (P Q R : Prop) (g : bool → nat), (p a) → (p b) → (q b) → ∃ x, p x ∧ q x)
+meta def x38 : expr := `(forall (a b c : ℕ) (p q : ℕ → Prop) (r : ℕ → ℕ → Prop) (P Q R : Prop) (g : bool → nat), (∃ x, p x ∧ r x x) → (∀ x, r x x → q x) → ∃ x, p x ∧ q x)
+meta def x39 : expr := `(forall (a b c : ℕ) (p q : ℕ → Prop) (r : ℕ → ℕ → Prop) (P Q R : Prop) (g : bool → nat), (∃ x, q x ∧ p x) → ∃ x, p x ∧ q x)
+meta def x40 : expr := `(forall (a b c : ℕ) (p q : ℕ → Prop) (r : ℕ → ℕ → Prop) (P Q R : Prop) (g : bool → nat), (∀ x, q x → p x) → (q a) → ∃ x, p x)
+meta def x41 : expr := `(forall (a b c : ℕ) (p q : ℕ → Prop) (r : ℕ → ℕ → Prop) (P Q R : Prop) (g : bool → nat), (∀ x, p x → q x → false) → (p a) → (p b) → (q b) → false)
+meta def x42 : expr := `(forall (a b c : ℕ) (p q : ℕ → Prop) (r : ℕ → ℕ → Prop) (P Q R : Prop) (g : bool → nat), (∀ x, p x) → (∀ x, p x → q x) → ∀ x, q x)
+meta def x43 : expr := `(forall (a b c : ℕ) (p q : ℕ → Prop) (r : ℕ → ℕ → Prop) (P Q R : Prop) (g : bool → nat), (∃ x, p x) → (∀ x, p x → q x) → ∃ x, q x)
+meta def x44 : expr := `(forall (a b c : ℕ) (p q : ℕ → Prop) (r : ℕ → ℕ → Prop) (P Q R : Prop) (g : bool → nat), (¬ ∀ x, ¬ p x) → (∀ x, p x → q x) → (∀ x, ¬ q x) → false)
+meta def x45 : expr := `(forall (a b c : ℕ) (p q : ℕ → Prop) (r : ℕ → ℕ → Prop) (P Q R : Prop) (g : bool → nat), (p a) → (p a → false) → false)
+
+meta def tests : list expr :=
+[ x01, x02, x03, x04, x05, x06, x07, x08, x09, x10,
+  x11, x12, x13, x14, x15, x16, x17, x18, x19, x20 ]
+  -- x21, x22, x23, x24, x25, x26, x27, x28, x29, x30 ]
+  --x31, x32, x33, x34, x35, x36, x37, x38, x39, x40,
+  --x41, x42, x43, x44, x45 ]
+
+open tactic
+
+meta def batch_test (t : tactic unit) : nat → list expr → tactic unit
+| _   []          := tactic.triv
+| idx (exp::exps) :=
+  ( (do gs ← tactic.get_goals,
+       g ← tactic.mk_meta_var exp,
+       tactic.set_goals (g::gs), t) <|>
+    (trace (("Failed ex " : format) ++ format.of_nat idx) >> tactic.skip)) >>
+  batch_test (idx+1) exps
+
+set_option profiler true
+
+example : true :=
+by do batch_test leancop 1 tests
+
+#exit
+
+#exit
+section
+
+
+
+end
+
+end
+
+section
+
+variables a b c d : Prop
+
+
+end
+
+section
+
+variables (a b c : ℕ) (p q : ℕ → Prop) (r : ℕ → ℕ → Prop) (P Q R : Prop) (g : bool → nat)
+
+
+end
+
+section
+
+  variables a b c d : Prop
+  variables (p q : ℕ → Prop) (r : ℕ → ℕ → Prop)
+
+  example : (¬ (a → b ∨ c)) → (¬ (b ∨ ¬ c)) → false := by leancop
+  example : (a → b ∨ c) → (¬ b) → a → c := by leancop
+
+end
