src/tactic/fol/foo.pl
@@ -1,0 +1,5 @@
+foo(X) :- not(X == 0).
+
+bar(X, Y) :- include(foo, X, Y).
+
+quz(L, M) :- maplist(bar, L, M).
