src/tactic/fol/leancop.pl
@@ -1,0 +1,59 @@
+#!/usr/bin/env swipl
+
+:- initialization(main, main).
+:- style_check(-singleton).
+
+:- [parse].
+:- [print].
+
+isPoint(-!).
+
+removePoint(X, Y) :- exclude(isPoint, X, Y).
+
+removePoints(P, Q) :- maplist(removePoint, P, Q).
+
+prove(Mat, PathLim, Used) :-
+     append(MatA, [Cla |MatB ], Mat),
+     \+member(-_,Cla),
+     append(MatA, MatB, Mat1),
+     prove([!], [[-! | Cla] | Mat1], [], PathLim, Used).
+
+prove(Mat, PathLim, Used) :-
+     \+ground(Mat), PathLim1 is PathLim+1, prove(Mat, PathLim1, Used).
+
+prove([], _, _, _, []).
+
+prove([Lit | Cla], Mat, Path, PathLim, Used) :-
+  (-NegLit=Lit ; -Lit=NegLit) ->
+  (
+    (
+      member(NegL,Path),
+      unify_with_occurs_check(NegL, NegLit),
+      Used1 = []
+    )
+    ;
+    (
+      append(MatA,[Cla1|MatB],Mat), copy_term(Cla1,Cla2),
+      append(ClaA,[NegL|ClaB],Cla2),
+      unify_with_occurs_check(NegL,NegLit),
+      append(ClaA,ClaB,Cla3),
+      (
+        Cla1==Cla2 ->
+          append(MatB,MatA,Mat1)
+          ;
+          length(Path,K), K<PathLim,
+          append(MatB,[Cla1|MatA],Mat1)
+      ),
+      prove(Cla3,Mat1,[Lit|Path],PathLim, Used2),
+      Used1 = [Cla2 | Used2]
+    )
+  ),
+  prove(Cla, Mat, Path, PathLim, Used3),
+  append(Used1, Used3, Used).
+
+main([MS|_]) :-
+  parseMat(MS, M),
+  prove(M, 1, U),
+  removePoints(U, P),
+  printMat(P, S),
+  write(S).
