src/tactic/fol/leancop_bak.pl
@@ -1,0 +1,162 @@
+#!/usr/bin/env swipl
+
+:- initialization(main, main).
+
+:- set_prolog_flag(optimise,true).
+
+:- dynamic(pathlim/0), dynamic(lit/4).
+
+:- style_check(-singleton).
+
+assignVar([], 0, V, [V]).
+
+assignVar([], N, V, [W|Vs]) :-
+  M is N - 1,
+  assignVar([], M, V, Vs).
+
+assignVar([V|Vs], 0, V, [V|Vs]).
+
+assignVar([V|Vs], N, W, [V|Ws]) :-
+  M is N - 1,
+  assignVar(Vs, M, W, Ws).
+
+parseLit(["-" | Ts], Vs, -L, Ts1, Vs1) :-
+  parseLit(Ts, Vs, L, Ts1, Vs1).
+
+parseLit(["S" | [T | Ts]], Vs, (N), Ts, Vs) :-
+  number_string(N, T).
+
+parseLit(["V" | [T | Ts]], Vs, L, Ts, Vs1) :-
+  number_string(N, T), assignVar(Vs, N, L, Vs1).
+
+parseLit(["(" | Ts], Vs, app(L1, L2), Ts2, Vs2) :-
+  parseLit(Ts,  Vs,  L1, Ts1, Vs1),
+  parseLit(Ts1, Vs1, L2, [")" | Ts2], Vs2).
+
+parseCla(Ts, Vs, [L | C], Ts2, Vs2) :-
+  parseLit(Ts, Vs, L, Ts1, Vs1),
+  parseCla(Ts1, Vs1, C, Ts2, Vs2).
+
+parseCla(["|" | Ts], Vs, [], Ts, Vs).
+
+% parseCla(["[" | Ts], C, Ts1) :-
+%   parseClaCore(Ts, [], C, Ts1, _).
+
+parseMatCore(Ts, [C | M]) :-
+  parseCla(Ts, [], C, Ts1, _),
+  parseMatCore(Ts1, M).
+
+parseMatCore([], []).
+
+parseMat(MS, M) :-
+  split_string(MS, " ", " ", Ts),
+  parseMatCore(Ts, M).
+
+%%% prove matrix M / formula F
+
+prove(F,Proof) :- prove2(F,[cut,comp(7)],Proof).
+
+prove2(F,Set,Proof) :-
+    (F=[_|_] -> M=F ; make_matrix(F,M,Set)),
+    retractall(lit(_,_,_,_)), (member([-(#)],M) -> S=conj ; S=pos),
+    assert_clauses(M,S), prove(1,Set,Proof).
+
+prove(PathLim,Set,Proof) :-
+    \+member(scut,Set) -> prove([-(#)],[],PathLim,[],Set,[Proof]) ;
+    lit(#,_,C,_) -> prove(C,[-(#)],PathLim,[],Set,Proof1),
+    Proof=[C|Proof1].
+
+prove(PathLim,Set,Proof) :-
+    member(comp(Limit),Set), PathLim=Limit -> prove(1,[],Proof) ;
+    (member(comp(_),Set);retract(pathlim)) ->
+    PathLim1 is PathLim+1, prove(PathLim1,Set,Proof).
+
+%%% leanCoP core prover
+
+prove([],_,_,_,_,[]).
+
+prove([Lit|Cla],Path,PathLim,Lem,Set,Proof) :-
+    Proof=[[[NegLit|Cla1]|Proof1]|Proof2],
+    \+ (member(LitC,[Lit|Cla]), member(LitP,Path), LitC==LitP),
+    (-NegLit=Lit;-Lit=NegLit) ->
+       ( member(LitL,Lem), Lit==LitL, Cla1=[], Proof1=[]
+         ;
+         member(NegL,Path), unify_with_occurs_check(NegL,NegLit),
+         Cla1=[], Proof1=[]
+         ;
+         lit(NegLit,NegL,Cla1,Grnd1),
+         unify_with_occurs_check(NegL,NegLit),
+         ( Grnd1=g -> true ; length(Path,K), K<PathLim -> true ;
+           \+ pathlim -> assert(pathlim), fail ),
+         prove(Cla1,[Lit|Path],PathLim,Lem,Set,Proof1)
+       ),
+       ( member(cut,Set) -> ! ; true ),
+       prove(Cla,Path,PathLim,[Lit|Lem],Set,Proof2).
+
+%%% write clauses into Prolog's database
+
+assert_clauses([],_).
+assert_clauses([C|M],Set) :-
+    (Set\=conj, \+member(-_,C) -> C1=[#|C] ; C1=C),
+    (ground(C) -> G=g ; G=n), assert_clauses2(C1,[],G),
+    assert_clauses(M,Set).
+
+assert_clauses2([],_,_).
+assert_clauses2([L|C],C1,G) :-
+    assert_renvar([L],[L2]), append(C1,C,C2), append(C1,[L],C3),
+    assert(lit(L2,L,C2,G)), assert_clauses2(C,C3,G).
+
+assert_renvar([],[]).
+assert_renvar([F|FunL],[F1|FunL1]) :-
+    ( var(F) -> true ; F=..[Fu|Arg], assert_renvar(Arg,Arg1),
+      F1=..[Fu|Arg1] ), assert_renvar(FunL,FunL1).
+
+depoint([], []).
+depoint([(#) | C], D) :-
+  depoint(C, D).
+depoint([L | C], [L | D]) :-
+  depoint(C, D).
+
+flatten([C], [D]) :- depoint(C, D).
+
+flatten([C, P], [D | M]) :-
+  depoint(C, D),
+  flatten(P, M).
+
+formatLit(-A, S) :-
+  formatLit(A, AS),
+  string_concat("- ", AS, S).
+
+formatLit(app(A, B), S) :-
+  formatLit(A, AS),
+  formatLit(B, BS),
+  string_concat("( ", AS, PAS),
+  string_concat(PAS, " ", PASS),
+  string_concat(BS, " )", BSS),
+  string_concat(PASS, BSS, S).
+
+formatLit(N, S) :- atom_string(N, S).
+
+formatCla([], "").
+
+formatCla([L | C], S) :-
+  formatLit(L, LS),
+  formatCla(C, CS),
+  string_concat(LS, " ", LSS),
+  string_concat(LSS, CS, S).
+
+formatMat([], "").
+
+formatMat([C | M], S) :-
+  formatCla(C, CS),
+  formatMat(M, MS),
+  string_concat(CS, "| ", CSS),
+  string_concat(CSS, MS, S).
+
+main([MS|_]) :-
+  parseMat(MS, M),
+  prove(M, P),
+  flatten(P, N),
+  formatMat(N, S),
+  write(S).
+  % write(M).
