src/tactic/fol/parse.pl
@@ -1,0 +1,40 @@
+assignVar([], 0, V, [V]).
+
+assignVar([], N, V, [W|Vs]) :-
+  M is N - 1,
+  assignVar([], M, V, Vs).
+
+assignVar([V|Vs], 0, V, [V|Vs]).
+
+assignVar([V|Vs], N, W, [V|Ws]) :-
+  M is N - 1,
+  assignVar(Vs, M, W, Ws).
+
+parseLit(["-" | Ts], Vs, -L, Ts1, Vs1) :-
+  parseLit(Ts, Vs, L, Ts1, Vs1).
+
+parseLit(["S" | [T | Ts]], Vs, (N), Ts, Vs) :-
+  number_string(N, T).
+
+parseLit(["V" | [T | Ts]], Vs, L, Ts, Vs1) :-
+  number_string(N, T), assignVar(Vs, N, L, Vs1).
+
+parseLit(["(" | Ts], Vs, app(L1, L2), Ts2, Vs2) :-
+  parseLit(Ts,  Vs,  L1, Ts1, Vs1),
+  parseLit(Ts1, Vs1, L2, [")" | Ts2], Vs2).
+
+parseCla(Ts, Vs, [L | C], Ts2, Vs2) :-
+  parseLit(Ts, Vs, L, Ts1, Vs1),
+  parseCla(Ts1, Vs1, C, Ts2, Vs2).
+
+parseCla(["|" | Ts], Vs, [], Ts, Vs).
+
+parseMatCore(Ts, [C | M]) :-
+  parseCla(Ts, [], C, Ts1, _),
+  parseMatCore(Ts1, M).
+
+parseMatCore([], []).
+
+parseMat(MS, M) :-
+  split_string(MS, " ", " ", Ts),
+  parseMatCore(Ts, M).
