src/tactic/fol/print.pl
@@ -1,0 +1,29 @@
+printLit(-A, S) :-
+  printLit(A, AS),
+  string_concat("- ", AS, S).
+
+printLit(app(A, B), S) :-
+  printLit(A, AS),
+  printLit(B, BS),
+  string_concat("( ", AS, PAS),
+  string_concat(PAS, " ", PASS),
+  string_concat(BS, " )", BSS),
+  string_concat(PASS, BSS, S).
+
+printLit(N, S) :- atom_string(N, S).
+
+printCla([], "").
+
+printCla([L | C], S) :-
+  printLit(L, LS),
+  printCla(C, CS),
+  string_concat(LS, " ", LSS),
+  string_concat(LSS, CS, S).
+
+printMat([], "").
+
+printMat([C | M], S) :-
+  printCla(C, CS),
+  printMat(M, MS),
+  string_concat(CS, "| ", CSS),
+  string_concat(CSS, MS, S).
